MiniKyoLean/MiniUnsafeLaws.lean
@@ -1,0 +1,52 @@
+import MiniKyoLean.MiniUnsafe
+
+
+/-
+
+  * Left Identity
+  *   - pure(a).flatMap(f) ≡ f(a)
+  *
+  * Right Identity
+  *   - m.flatMap(pure) ≡ m
+  *
+  * Associativity
+  *   - m.flatMap(f).flatMap(g) ≡ m.flatMap(x => f(x).flatMap(g))
+  *
+  * Pure Handling
+  *   - handle(tag, pure(value), f) ≡ pure(value)
+  *
+  * Effect Handling
+  *   - handle(tag1, suspend(tag2, input, cont), f) ≡ handle(tag1, f(input, cont), f) where tag1 ≡ tag2
+  *
+  * Handler Rotation
+  *   - handle(tag1, suspend(tag2, input, cont), f) ≡ suspend(tag2, input, x => handle(tag1, cont(x), f)) where tag1 ≠ tag2
+
+
+ -/
+
+open kernel
+open kernel.Kyo
+
+theorem leftIdentity {A B : Type} (a : A) (f : A -> Kyo B) : ((pure a).flatMap f) = f a :=
+  rfl
+
+theorem rightIdentity {A : Type} (m : Kyo A) : m.flatMap pure = m :=
+  match m with
+  | Kyo.Pure a => rfl
+  | Suspend tag input cont =>
+    by
+      -- unfold flatMap
+      simp [flatMap]
+      funext o
+      exact rightIdentity (cont o)
+
+theorem associativity
+  {A B C : Type} (m : Kyo A) (f : A -> Kyo B) (g : B -> Kyo C)
+  : (m.flatMap f).flatMap g = m.flatMap (fun x => (f x).flatMap g) :=
+  match m with
+  | Kyo.Pure a => rfl
+  | Suspend tag input cont =>
+    by
+      simp [flatMap]
+      funext o
+      exact associativity (cont o) f g
